:PROPERTIES:
:ID:       4a4be2c5-36c5-4aeb-a62a-3535901b6129
:END:
#+title: De Morgan's Laws
#+filetags: logic

* Definition
#+begin_quote
If \(\square\) and \(\triangle\) are [[id:87704c09-b23d-4980-ab11-0a5f839ebf59][operations]] on a set \(X\) and \({}^{\circ}\) is a unary operation on \(X\) then De Morgen's Law states that
\begin{equation*}
(x \square y)^{\circ} = x^{\circ}\triangle y^{\circ}
\end{equation*}
#+end_quote

* Applied to [[id:56ae2cf4-a426-46fd-82eb-9acb3c8512ba][Sets]]
\((E\cup F)^{c} = E^{c}\cap F^{c}\) and \((E \cap F)^{c} = E^{c}\cup F^{c}\)

** In General
#+begin_quote
If \(U\) is a universal set then for any subsets \(A_1, A_2,\ldots,A_n\) then
\begin{equation*}
\overline{\bigcup_{k=1}^nA_k} = \bigcap_{k=1}^n\overline{A_{k}}
\end{equation*}

This can be proved by [[id:c0407dfb-dd46-488d-88e3-25733c215325][Mathematical Induction]] on \(n\).
#+end_quote

* Applied to [[id:c320994c-b8c2-4d38-8954-d75f1c8aa022][Logical Operators]]
\(\neg(E \vee F) = (\neg E) \wedge (\neg F)\) and \(\neg(E \wedge F) = (\neg E) \vee (\neg F)\)

** Example
The statement "It is not the case that Bob ate pizza at lunch and then went for a walk", would be equivalent to "Either Bob didn't eat pizza for lunch or Bob didn't go for a walk".
