:PROPERTIES:
:ID:       f9cfe2d4-3f37-42f7-82be-91105f5caeb0
:ROAM_ALIASES: "Addition Principle"
:END:
#+title: Inclusion-exclusion Principle
#+filetags: probability_propositions fundamentals counting

* Definition
For any two events \(E\) and \(F\) in the sample space,
\begin{equation*}
P(E\cup F) = P(E) + P(F) - P(E\cap F)
\end{equation*}
and for any two finite sets \(E\) and \(F\) which are subsets of the universal set \(U\),
\begin{equation*}
|E\cup F| = |E| + |F| - |E\cap F|
\end{equation*}

** For 3 events
\begin{equation*}
P(E\cup F\cup G) = P(E) + P(F) + P(G) \\
- P(E\cap F) - P(E\cap G) - P(F \cap G) + P(E \cap F \cap G)
\end{equation*}

* Proof
$E \cup F = E \cup E^c \cap F$, with $E$ and $E^c \cap F$ [[id:b804e882-b52f-49fd-a577-bcae712bbb75][mutually exclusive]].
\begin{equation*}
P(E \cup F) = P(E) + P(E^c \cap F) \quad [\text{axiom 3}]
\end{equation*}
$F = EF \cup E^c \cap F$, with $EF$ and $E^c \cap F$ mutually exclusive.
\begin{equation*}
P(F) = P(EF) + P(E^c \cap F) \quad [\text{axiom 3}]
\end{equation*}
Therefore,
\begin{equation*}
P(E \cup F) = P(E) + P(F) - P(EF).
\end{equation*}
