:PROPERTIES:
:ID:       d633683f-d6eb-4271-9717-55fd95628cfc
:END:
#+title: Complement Rule
#+filetags: probability_propositions

* Proposition
For any [[id:33838eb4-aa50-4794-baa1-637ddea744ad][event]] \(E\) in a [[id:33838eb4-aa50-4794-baa1-637ddea744ad][sample space]] \(S\),
\begin{equation*}
P(E^{c}) = 1 - P(E)
\end{equation*}

* Proof
We know that $S = E \cup E^c$, with $E$ and $E^c$ [[id:b804e882-b52f-49fd-a577-bcae712bbb75][mutually exclusive]].
\begin{equation*}
P(S) = P(E \cup E^c)
\end{equation*}
\begin{equation*}
1 = P(E) + P(E^c) \quad [\text{axioms 2 and 3}]
\end{equation*}
\begin{equation*}
\therefore P(E^c) = 1 - P(E).
\end{equation*}
