:PROPERTIES:
:ID:       c0407dfb-dd46-488d-88e3-25733c215325
:END:
#+title: Mathematical Induction
#+filetags: logic

* Definition
#+begin_quote
Given any [[id:ac356044-060c-4b67-84f2-6361c9c574bb][predicate]] over \(\mathbb{N}\), say \(P\) then if \(P(0)\) is true and \(P(n) \Rightarrow P(n+1)\) is true for any \(n\in\mathbb{N}\) then \(P(n)\) is true for all \(n\in\mathbb{N}\).

\begin{equation*}
P(0) \wedge \forall n\in\mathbb{N} \left[P(n) \Rightarrow P(n+1)\right] \equiv \forall n\in\mathbb{N} [P(n)]
\end{equation*}
#+end_quote

* Principle of Mathematical Induction
Suppose \(\alpha(n)\) is a [[id:ac356044-060c-4b67-84f2-6361c9c574bb][var-statement]] about natural numbers \(n\).
If we can know that
1. \(\alpha(1)\) is true
2. for any \(k\in\mathbb{N}\), \(\alpha(k)\Rightarrow\alpha(k+1)\) is true

  then \(\alpha(n)\) is true for all \(n\in\mathbb{N}\)

This is equivalent to the [[id:39937c5a-c5a2-4b90-b87a-e6250150d607][Well-ordering Principle]] of \(\mathbb{N}\)

** Motivation
Say (1) and (2) hold for some statement \(\alpha(n)\) over \(\mathbb{N}\)
- by (1) \(\alpha(1)\) true
- by (2) \(\alpha(1)\Rightarrow\alpha(2)\) so \(\alpha(2)\) true
- by (2) \(\alpha(2)\Rightarrow\alpha(3)\) so \(\alpha(3)\) true
- \(\cdots\)

* Proof by Induction
- Prove \(\alpha(1)\) is true
- We let \(k\in\mathbb{N}\), assume \(\alpha(k)\) is true
- Prove that \(\alpha(k+1)\) is true

* Examples
[[file:images/induction-1.png]]
[[file:images/induction-2.png]]
