:PROPERTIES:
:ID:       6d130bdd-0096-4d4c-a150-2855608486f1
:END:
#+title: Summation Index Shift

* Definition
#+begin_quote
Let \(f(i)\) be some function of \(i\), then for any \(n\in\mathbb{N}\)
\begin{equation*}
\sum_{i=0}^nf(i) = \sum_{i=1}^{n+1}f(i-1)
\end{equation*}
#+end_quote

* Proof
Let \(f\) be any function on \(\mathbb{N}\cup\{0\}\).

** Base case (\(n = 0\)):

\(\sum_{i=0}^0f(i) = f(0)\)

\(\sum_{i=1}^1f(i-1) = f(0)\)

** Induction step:
Let \(k\in\mathbb{N}\cup\{0\}\) and suppose \(\sum_{i=0}^kf(i) = \sum_{i=1}^{k+1}f(i-1)\)
\begin{align*}
\sum_{i=0}^{k+1}f(i) &= \left(\sum_{i=0}^{k}f(i)\right) + f(k + 1) \\
&= \left(\sum_{i=1}^{k+1}f(i-1)\right) + f(k+1) \text{ by I.H.} \\
&= \left(\sum_{i=1}^{k+1}f(i-1)\right) + f\left((k+1+1)-1\right) \\
&= \sum_{i=1}^{(k+1)+1}f(i-1)
\end{align*}

By [[id:c0407dfb-dd46-488d-88e3-25733c215325][Mathematical Induction]], \( \sum_{i=0}^nf(i) = \sum_{i=1}^{n+1}f(i-1)\) for all \(n\in\mathbb{N}\cup\{0\}\)
